WIP: de/serialize Mutations Input

AwsCryptographicMaterialProviders/dafny/AwsCryptographyKeyStoreAdmin/src/MutationStateStructures.dfy
@@ -68,7 +68,7 @@ module {:options "/functionSyntax:4" } MutationStateStructures {
     CreateTime: string,
     ExclusiveStartKey: MutationIndexUtils.ExclusiveStartKey := Option.None,
     UUID: string,
-    Input: seq<uint8>,
+    Input: Types.Mutations,
     CommitmentCiphertext: seq<uint8>,
     IndexCiphertext: seq<uint8>
   )
@@ -162,6 +162,46 @@ module {:options "/functionSyntax:4" } MutationStateStructures {
     // Note: no Extract method
   }
 
+  function InputMutationsToJson(
+    Mutations: Types.Mutations
+  ): (output: JSONValues.JSON)
+  {
+    var ec: JSONValues.JSON :=
+      if Mutations.TerminalEncryptionContext.Some?
+      then EncryptionContextStringToJSON(Mutations.TerminalEncryptionContext.value)
+      else JSONValues.Null;
+    var kms: JSONValues.JSON :=
+      if Mutations.TerminalKmsArn.Some?
+      then JSONValues.JSON.String(Mutations.TerminalKmsArn.value)
+      else JSONValues.Null;
+    var inputJson
+      := JSONValues.Object([(AWS_CRYPTO_EC, ec), (KMS_FIELD, kms)]);
+    inputJson
+  }
+  
+  function InputMutationsFromJson(
+    MutationsJson: JSONValues.JSON
+  ): (output: Types.Mutations)
+    requires MutationsJson.Object? && |MutationsJson.obj| == 2
+    requires MutationsJson.obj[0].1.Object? ==>
+      (var EncryptionContext := MutationsJson.obj[0].1;
+      && (forall p <- EncryptionContext.obj :: p.1.String?)
+      && (|set p <- EncryptionContext.obj :: p.0| == |EncryptionContext.obj|))
+  {
+    var ec: Option<KeyStoreTypes.EncryptionContextString> :=
+      if MutationsJson.obj[0].1.Object?
+      then Some(JSONToEncryptionContextString(MutationsJson.obj[0].1))
+      else None;
+    var kms: Option<string> :=
+      if MutationsJson.obj[1].1.String?
+      then Some(MutationsJson.obj[1].1.str)
+      else None;
+    var input
+      := Types.Mutations(
+      TerminalKmsArn := kms,
+      TerminalEncryptionContext := ec);
+    input
+  }
 
   function SerializeMutableBranchKeyProperties(
     MutationToApply: MutationToApply
@@ -181,6 +221,8 @@ module {:options "/functionSyntax:4" } MutationStateStructures {
              (KMS_FIELD, JSONValues.JSON.String(MutationToApply.Terminal.kmsArn))
            ]);
 
+    var InputJson := InputMutationsToJson(MutationToApply.Input);
+      
     var originalBytes :- JSON.Serialize(OriginalJson).MapFailure(
                            (e: JSONErrors.SerializationError)
                            => Types.KeyStoreAdminException(
@@ -188,7 +230,11 @@ module {:options "/functionSyntax:4" } MutationStateStructures {
     var terminalBytes :- JSON.Serialize(TerminalJson).MapFailure(
                            (e: JSONErrors.SerializationError)
                            => Types.KeyStoreAdminException(
-                               message := "Could not JSON Serialize state: terminal properties. " + e.ToString()));
+                           message := "Could not JSON Serialize state: terminal properties. " + e.ToString()));
+    var inputBytes :- JSON.Serialize(InputJson).MapFailure(
+                           (e: JSONErrors.SerializationError)
+                           => Types.KeyStoreAdminException(
+                               message := "Could not JSON Serialize Input. " + e.ToString()));
     var commitment := KeyStoreTypes.MutationCommitment(
                         Identifier := MutationToApply.Identifier,
                         Original := originalBytes,
@@ -196,7 +242,7 @@ module {:options "/functionSyntax:4" } MutationStateStructures {
                         UUID := MutationToApply.UUID,
                         CreateTime := MutationToApply.CreateTime,
                         CiphertextBlob := MutationToApply.CommitmentCiphertext,
-                        Input := MutationToApply.Input
+                        Input := inputBytes
                       );
     var index := KeyStoreTypes.MutationIndex(
                    Identifier := MutationToApply.Identifier,
@@ -218,15 +264,20 @@ module {:options "/functionSyntax:4" } MutationStateStructures {
     var OriginalJson :- JSON.Deserialize(commitment.Original).MapFailure(
                           (e: JSONErrors.DeserializationError)
                           => Types.KeyStoreAdminException(
-                              message := "Could not JSON Deserialize state: original properties. " + e.ToString()));
+                              message := "Could not JSON Deserialize: original properties. " + e.ToString()));
 
     var TerminalJson :- JSON.Deserialize(commitment.Terminal).MapFailure(
                           (e: JSONErrors.DeserializationError)
                           => Types.KeyStoreAdminException(
-                              message := "Could not JSON Deserialize state: terminal properties. " + e.ToString()));
+                          message := "Could not JSON Deserialize: terminal properties. " + e.ToString()));
+    var InputJson :- JSON.Deserialize(commitment.Input).MapFailure(
+                          (e: JSONErrors.DeserializationError)
+                          => Types.KeyStoreAdminException(
+                              message := "Could not JSON Deserialize: Input. " + e.ToString()));                          
 
     :- MutablePropertiesJson?(OriginalJson);
     :- MutablePropertiesJson?(TerminalJson);
+    :- MutationsInputJson?(InputJson);
 
     Success(
       MutationToApply(
@@ -244,7 +295,7 @@ module {:options "/functionSyntax:4" } MutationStateStructures {
         ExclusiveStartKey := MutationIndexUtils.PageIndexToExclusiveStartKey(index.PageIndex),
         CommitmentCiphertext := commitment.CiphertextBlob,
         IndexCiphertext := index.CiphertextBlob,
-        Input := commitment.Input
+        Input := InputMutationsFromJson(InputJson)
       ))
   }
 
@@ -304,6 +355,75 @@ module {:options "/functionSyntax:4" } MutationStateStructures {
     Outcome.Pass
   }
 
+  function MutationsInputJson?(
+    DeserializedMutations: JSONValues.JSON
+  ): (output: Outcome<Types.Error>)
+  {
+    :- NeedOutcome(
+         DeserializedMutations.Object? && |DeserializedMutations.obj| == 2,
+         () => Types.KeyStoreAdminException( message := ERROR_PRFX + "There MUST not be more than two objects.")
+       );
+    :- NeedOutcome(
+         DeserializedMutations.obj[0].0 == AWS_CRYPTO_EC,
+         () => Types.KeyStoreAdminException( message := ERROR_PRFX + "First Key MUST be Encryption Context.")
+       );
+    :- NeedOutcome(
+         DeserializedMutations.obj[1].0 == KMS_FIELD,
+         () => Types.KeyStoreAdminException( message := ERROR_PRFX + "Second Key MUST be KMS ARN.")
+       );
+    :- NeedOutcome(
+         DeserializedMutations.obj[0].1.Object? || DeserializedMutations.obj[0].1.Null?,
+         () => Types.KeyStoreAdminException(
+             message := ERROR_PRFX + "Value for `" + AWS_CRYPTO_EC + "` MUST be an object or Null.")
+       );
+    :- NeedOutcome(
+         DeserializedMutations.obj[1].1.String? || DeserializedMutations.obj[1].1.Null?,
+         () => Types.KeyStoreAdminException(
+             message := ERROR_PRFX + "Value for `" + KMS_FIELD + "` MUST be a string or Null.")
+        );
+
+    // For the input, I do not think we care if the KMS ARN is valid         
+    // :- NeedOutcome(
+    //      KmsArn.ValidKmsArn?(DeserializedMutations.obj[1].1.str),
+    //      () => Types.KeyStoreAdminException( message := ERROR_PRFX + "KMS ARN that has been deserialized is invalid.")
+    //    );
+    NullableEncryptionContextJson?(DeserializedMutations.obj[0].1)
+  }
+
+  function NullableEncryptionContextJson?(
+    NullableEncryptionContext: JSONValues.JSON
+  ): (output: Outcome<Types.Error>)
+    requires NullableEncryptionContext.Object? || NullableEncryptionContext.Null?
+  {
+    if NullableEncryptionContext.Null?
+      then Outcome.Pass
+      else EncryptionContextJson?(NullableEncryptionContext)
+  }
+
+  function EncryptionContextJson?(
+    EncryptionContextJson: JSONValues.JSON
+  ): (output: Outcome<Types.Error>)
+    requires EncryptionContextJson.Object?
+  {
+    :- NeedOutcome(
+         forall p <- EncryptionContextJson.obj :: p.1.String?,
+         () => Types.KeyStoreAdminException( message := ERROR_PRFX + "Member of Encryption Context cannot be deserialized.")
+       );
+
+    var EncryptionContextKeys := set p <- EncryptionContextJson.obj :: p.0;
+    :- NeedOutcome(
+         |EncryptionContextKeys| == |EncryptionContextJson.obj|,
+         () => Types.KeyStoreAdminException(
+             message := ERROR_PRFX + "Size of Encryption Context keys is not equal to size of Encryption Context values. ")
+       );
+    :- NeedOutcome(
+         Structure.BRANCH_KEY_RESTRICTED_FIELD_NAMES !! EncryptionContextKeys,
+         () => Types.KeyStoreAdminException(
+             message := "Invalid Mutation Token: MUST NOT model Item specific fields!")
+       );
+    Outcome.Pass
+  }
+  
   // Quality of life proof that a correctly constructed JSON object,
   // will in fact go into a Dafny Map
   lemma LemmaJSONObjectCanConvertToDafnyMap(
